chmaps mostly done (paused on proofs in file to update automation, which is not done

KeyManagement/IdealWorld.v
@@ -20,25 +20,33 @@ From Coq Require Import String Bool.Sumbool Logic.
 Require Import MyPrelude.
 
 (* Module Foo <: EMPTY. End Foo. *)
+
 (* Module Import SN := SetNotations(Foo). *)
 
-Require Import Common Maps Messages.
+Require Import Common ChMaps Maps Messages.
+Import ChNotation.
+
+
 Require Messages.
 Set Implicit Arguments.
 
-Definition channel_id := nat.
+Definition channel_id := ChMaps.channel_id.
 
 Record permission := construct_permission
   { read : bool ;
     write : bool }.
 
+(* The user's list of allowed channels, the nat corresponds to the nat in Single n *)
 Definition permissions := NatMap.t permission.
+Definition perm_id := nat.
 
 Definition creator_permission := construct_permission true true.
 
+(* this is what you send to a different user to grant access, later restricted to 
+   Single channel ids *)
 Record access := construct_access
                    { ch_perm : permission ;
-                     ch_id : channel_id }.
+                     ch_id : perm_id }.
 
 Module IW_message <: GRANT_ACCESS.
   Definition access := access.
@@ -48,14 +56,40 @@ Module message := Messages(IW_message).
 Import message.
 Export message.
 
-(* shouldn't this be just Permissions ? *)
-Definition channels := NatMap.t (list (sigT message)).
+(* now it's an inductive channel ID map *)
+(* channels are created when:
+   1) the universe is initialized with a non-empty map
+   2) a user generates a new channel
+   3) a user sends or receives on a channel intersection for the first time *)
+Definition channels := ChMap.t (list (sigT message)).
+
+Definition perm_intersection (perm1 perm2 : permission) :=
+  match (perm1, perm2) with
+  | (construct_permission rb1 wb1, construct_permission rb2 wb2) =>
+    construct_permission (andb rb1 rb2) (andb wb1 wb2)
+  end.
+
+Definition check_perm (ch : channel_id) (ps : permissions) (target : permission) : Prop :=
+  match ch with
+  | Single n =>
+    match (ps $? n) with
+    | Some p' => p' = target
+    | None => False
+    end
+  | Intersection n1 n2 =>
+    match (ps $? n1, ps $? n2) with
+    | (Some p1, Some p2) => (perm_intersection p1 p2) = target
+    | _ => False
+    end
+  end.
+
 
 Inductive cmd_type :=
 | ChannelId
 | Base (t : type)
 | Message (t : type)
 .
+
 Definition denote (t : cmd_type) :=
   match t with
   | ChannelId => channel_id
@@ -105,39 +139,37 @@ Record user A :=
 Record universe A :=
   construct_universe {
       channel_vector : channels (* fmap channel_id channels *)
-    ; users : user_list (user A)
+      ; users : user_list (user A)
     }.
-
-(* write as inductive relation *)
-Fixpoint chs_search {A} (m : message A) : list (channel_id * permission) :=
-  match m with
-  | Permission (construct_access p id) => [(id, p)]
-  | Content _ => []
-  | MsgPair m1 m2 => chs_search m1 ++ chs_search m2        
-  end.
 
 Inductive permission_subset : permission -> permission -> Prop :=
 | ReadWriteCase : forall p2,
     permission_subset p2 (construct_permission true true)
 | WriteCase : forall b,
     permission_subset (construct_permission false b) (construct_permission false true)
-| ReadCase : forall b,
+| ReadCase : forall b, 
     permission_subset (construct_permission b false) (construct_permission true false).
 
-Definition msg_permissions_valid {A} (m : message A) ps : Prop :=
-  List.Forall
-    (fun '(id, ps_sent) =>
-      match ps $? id with
-      | Some p => permission_subset ps_sent p
-      | None => False
-      end)
-    (chs_search m).
-    
+Inductive screen_msg : forall A, permissions -> message A -> Prop :=
+| ContentCase : forall c ps,
+    screen_msg ps (Content c)
+| PairCase : forall {A B} (m1 : message A) (m2 : message B) ps,
+    screen_msg ps m1
+    -> screen_msg ps m2
+    -> screen_msg ps (MsgPair m1 m2)
+| PermCase : forall p ps p_data,
+    ps $? p.(ch_id) = Some p_data
+    -> permission_subset p.(ch_perm) p_data
+    -> screen_msg ps (Permission p).
 
-Fixpoint add_chs_to_set (ks : list (channel_id * permission)) (ps : permissions) :=
-  match ks with
-  | [] => ps
-  | (id, perm) :: ks' => (add_chs_to_set ks' ps) $+ (id, perm)
+(* Definition perm_intersection p1 p2 := *)
+(*   match (p1, p2) with *)
+
+Fixpoint add_ps_to_set {A} (m : message A) (ps : permissions) : permissions :=
+  match m with
+  | Content _ => ps
+  | Permission p => ps $+ (p.(ch_id), p.(ch_perm))
+  | MsgPair m1 m2 => add_ps_to_set m1 (add_ps_to_set m2 ps)
   end.
 
 Inductive action : Type :=
@@ -156,51 +188,62 @@ Inductive lstep_user : forall A, ilabel -> channels * cmd A * permissions -> cha
 | LStepGen : forall cv ps n,
     lstep_user Silent (cv, Gen, ps) (cv, Return n, ps)
 | LStepCreateChannel : forall ch_id cv ps,
-    ~(In ch_id cv) ->
+    cv #? (Single ch_id) = None ->
     lstep_user Silent
                (cv, CreateChannel, ps)
-               (cv $+ (ch_id, []), @Return ChannelId ch_id, ps $+ (ch_id, creator_permission))
-| LStepSend : forall t cv (m : message t) ch_id ps ch_d b,
+               (cv #+ ((Single ch_id), []), @Return ChannelId (Single ch_id), ps $+ (ch_id, creator_permission))
+| LStepSend : forall t (cv : channels) (m : message t) ch_id ps ch_d b,
     ps $? ch_id = Some {| read := b ; write := true |} ->
-    cv $? ch_id = Some ch_d ->
-    msg_permissions_valid m ps ->
+    cv #? (Single ch_id) = Some ch_d ->
+    screen_msg ps m ->
     lstep_user
-      (Action (Output m ch_id cv ps))
-      (cv, Send m ch_id, ps)
-      (cv $+ (ch_id, ch_d ++ [existT _ _ m]), @Return (Base Unit) tt, ps)
+      (Action (Output m (Single ch_id) cv ps))
+      (cv, Send m (Single ch_id), ps) (cv #+ (Single ch_id, (ch_d ++ [existT _ _ m])), @Return (Base Unit) tt, ps)
+| LStepDualSend : forall t cv (m : message t) ch_id1 ch_id2 ps ch_d b ms,
+    check_perm (Intersection ch_id1 ch_id2) ps {| read := b ; write := true |}
+    -> screen_msg ps m
+    (* replace the following with non-option map lookup? *)
+    -> (cv #? (Intersection ch_id1 ch_id2) = Some ch_d -> ms = ch_d)
+      \/ (cv #? (Intersection ch_id1 ch_id2) = None -> ms = [])
+    -> lstep_user
+      (Action (Output m (Intersection ch_id1 ch_id2) cv ps))
+      (cv, Send m (Intersection ch_id1 ch_id2), ps)
+      (cv #+ (Intersection ch_id1 ch_id2, (ms ++ [existT _ _ m])), @Return (Base Unit) tt, ps)
 | LStepRecv : forall t (cv cv' : channels) ch_d ch_d' ps (m : message t) ch_id b,
-    cv $? ch_id = Some ch_d ->
-    ps $? ch_id = Some {| read := true ; write := b |} ->
-    ch_d = (existT _ _ m) :: ch_d' ->
-    cv' = cv $+ (ch_id, ch_d') ->
-    lstep_user
-      (Action (Input m ch_id cv ps))
-      (cv, Recv ch_id, ps)
-      (cv', @Return (Message t) m, add_chs_to_set (chs_search m) ps)
-.
+    cv #? ch_id = Some ch_d
+    -> check_perm ch_id ps {| read := true ; write := b |}
+    -> ch_d = (existT _ _ m) :: ch_d'
+    -> cv' = cv #+ (ch_id, ch_d')
+    -> lstep_user
+        (Action (Input m ch_id cv ps))
+        (cv, Recv ch_id, ps)
+        (cv', @Return (Message t) m, add_ps_to_set m ps).
 
+(* do the following two lemmas need to be extended for dual sends or do I need a total of 4 lemmas? *)
 Lemma LStepSend' : forall t cv cv' (m : message t) ch_id ps ch_d b,
     ps $? ch_id = Some {| read := b ; write := true |}
-    -> cv $? ch_id = Some ch_d
-    -> msg_permissions_valid m ps
-    -> cv' = cv $+ (ch_id, ch_d ++ [existT _ _ m])
-    -> lstep_user (Action (Output m ch_id cv ps)) (cv, Send m ch_id, ps) (cv', @Return (Base Unit) tt, ps).
+    -> cv #? (Single ch_id) = Some ch_d
+    -> screen_msg ps m
+    -> cv' = cv #+ (Single ch_id, (ch_d ++ [existT _ _ m]))
+    -> lstep_user (Action (Output m (Single ch_id) cv ps)) (cv, Send m (Single ch_id), ps) (cv', @Return (Base Unit) tt, ps).
 Proof.
   intros; subst; econstructor; eauto.
 Qed.
 
+Hint Extern 1 (check_perm _ _ _) => unfold check_perm; clean_map_lookups : core.
+
 Lemma LStepRecv' : forall t (cv cv' : channels) ch_d ch_d' ps ps' (m : message t) ch_id b,
-    cv $? ch_id = Some ch_d
+    cv #? (Single ch_id) = Some ch_d
     -> ps $? ch_id = Some {| read := true ; write := b |}
     -> ch_d = (existT _ _ m) :: ch_d'
-    -> ps' = add_chs_to_set (chs_search m) ps
-    -> cv' = cv $+ (ch_id, ch_d')
+    -> ps' = add_ps_to_set m ps
+    -> cv' = cv #+ (Single ch_id, ch_d')
     -> lstep_user
-        (Action (Input m ch_id cv ps))
-        (cv, Recv ch_id, ps)
+        (Action (Input m (Single ch_id) cv ps))
+        (cv, Recv (Single ch_id), ps)
         (cv', @Return (Message t) m, ps').
 Proof.
-  intros; subst; econstructor; eauto.
+  intros; subst; econstructor; eauto. 
 Qed.
 
 Inductive lstep_universe : forall {A}, universe A -> ilabel -> universe A -> Prop :=
