protocols/ExampleProtocols.v
@@ -21,6 +21,7 @@ From Coq Require Import
 Require Import
         MyPrelude
         Maps
+        ChMaps
         Messages
         Common
         Keys
@@ -91,13 +92,14 @@ Module SignPingSendProtocol.
   Section IW.
     Import IdealWorld.
 
-    Definition CH__A2B : channel_id := 0.
+    Definition CH__A2B : channel_id := (Single 0).
+    Definition perms_CH__A2B := 0.
 
-    Definition PERMS__a := $0 $+ (CH__A2B, {| read := true; write := true |}). (* writer *)
-    Definition PERMS__b := $0 $+ (CH__A2B, {| read := true; write := false |}). (* reader *)
+    Definition PERMS__a := $0 $+ (perms_CH__A2B, {| read := true; write := true |}). (* writer *)
+    Definition PERMS__b := $0 $+ (perms_CH__A2B, {| read := true; write := false |}). (* reader *)
 
     Definition ideal_univ_start :=
-      mkiU ($0 $+ (CH__A2B, [])) PERMS__a PERMS__b
+      mkiU (ChMap.add CH__A2B [] (@empty _)) PERMS__a PERMS__b
            (* user A *)
            ( n <- Gen
            ; _ <- Send (Content n) CH__A2B
@@ -169,13 +171,14 @@ Module EncPingSendProtocol.
   Section IW.
     Import IdealWorld.
 
-    Definition CH__A2B : channel_id := 0.
+    Definition CH__A2B : channel_id := Single 0.
+    Definition perms_CH__A2B := 0.
 
-    Definition PERMS__a := $0 $+ (CH__A2B, {| read := false; write := true |}). (* writer *)
-    Definition PERMS__b := $0 $+ (CH__A2B, {| read := true; write := false |}). (* reader *)
+    Definition PERMS__a := $0 $+ (perms_CH__A2B, {| read := false; write := true |}). (* writer *)
+    Definition PERMS__b := $0 $+ (perms_CH__A2B, {| read := true; write := false |}). (* reader *)
 
     Definition ideal_univ_start :=
-      mkiU ($0 $+ (CH__A2B, [])) PERMS__a PERMS__b
+      mkiU (ChMap.add CH__A2B [] (empty _)) PERMS__a PERMS__b
            (* user A *)
            ( n <- Gen
            ; _ <- Send (Content n) CH__A2B
